justificativa para o diagrama

lambda_x.v
@@ -2459,6 +2459,9 @@ Inductive betax : n_sexp -> n_sexp -> Prop :=
  | step_betax : forall (e1 e2: n_sexp) (x: atom),
      betax (n_app  (n_abs x e1) e2)  (n_sub e1 x e2).
 
+
+(* evitar renomeamento no caso step_abs2: 
+
 Inductive pix : n_sexp -> n_sexp -> Prop :=
 | step_var : forall (e: n_sexp) (y: atom),
     pix (n_sub (n_var y) y e) e
@@ -2467,7 +2470,20 @@ Inductive pix : n_sexp -> n_sexp -> Prop :=
 | step_abs1 : forall (e1 e2: n_sexp) (y : atom),
     pix (n_sub (n_abs y e1) y e2)  (n_abs y e1)
 | step_abs2 : forall (e1 e2: n_sexp) (x y: atom),
-    x <> y ->
+    x <> y -> x `notin` fv_nom e2 ->
+    pix (n_sub (n_abs x e1) y e2)  (n_abs x (n_sub e1 y e2))
+| step_app : forall (e1 e2 e3: n_sexp) (y: atom),
+    pix (n_sub (n_app e1 e2) y e3) (n_app (n_sub e1 y e3) (n_sub e2 y e3)). *)
+
+Inductive pix : n_sexp -> n_sexp -> Prop :=
+| step_var : forall (e: n_sexp) (y: atom),
+    pix (n_sub (n_var y) y e) e
+| step_gc : forall (e: n_sexp) (x y: atom),
+    x <> y -> pix (n_sub (n_var x) y e) (n_var x)
+| step_abs1 : forall (e1 e2: n_sexp) (y : atom),
+    pix (n_sub (n_abs y e1) y e2)  (n_abs y e1)
+| step_abs2 : forall (e1 e2: n_sexp) (x y: atom),
+    x <> y -> 
     pix (n_sub (n_abs x e1) y e2)  (n_abs x (n_sub e1 y e2))
 | step_app : forall (e1 e2 e3: n_sexp) (y: atom),
     pix (n_sub (n_app e1 e2) y e3) (n_app (n_sub e1 y e3) (n_sub e2 y e3)).
